src/spec/TLS13.Wire.Spec.fsti
@@ -15,6 +15,14 @@ val parse_supported_server_hello:
   input:B.bytes ->
   Tot (option H.server_hello)
 
+val parse_certificate_leaf_der:
+  input:B.bytes ->
+  Tot (option B.bytes)
+
+val parse_certificate_verify:
+  input:B.bytes ->
+  Tot (option H.certificate_verify)
+
 val serialize_supported_client_hello:
   hello:H.client_hello ->
   Tot B.bytes
